---
title:      Exercise 2.3-4
clrs:       [2, 3]
date:       2012-08-22 22:15
---

>Insertion sort can be expressed as a recursive procedure as follows. In order to sort $$A[1 . . n]$$, we recursively sort $$A[1 . . n−1]$$ and then insert A[n] into the sorted array $$A[1 . . n − 1]$$. Write a recurrence for the running time of this recursive version of insertion sort.

There are two steps in this recursive sorting algorithm:

1. Sort the sub-array $$A[1 .. n - 1]$$
2. Insert $$A[n]$$ into the sorted sub-array from step 1 in proper position

For $$n = 1$$, step 1 doesn't take any time as the sub-array is an empty array and step 2 takes constant time, i.e. the algorithm runs in $$\Theta(1)$$ time.

For $$n > 1$$, step 1 again calls for the recursion for $$n - 1$$ and step 2 runs in $$\Theta(n)$$ time.

So, we can write the recurrence as:

$$T(n) = \begin {cases}
    \Theta(1)               & \text { if } n = 1, \\
    T(n - 1) + \Theta(n)    & \text { if } n > 1
\end {cases}$$

<br/>
<hr/>
<div class="text-center"><h3>Additional Analysis</h3></div>
**Pseudo-code #1:** `RECURSE-INSERTION-SORT(A, n)`

{% highlight java linenos %}
if n > 1
    RECURSE-INSERTION-SORT(A, n - 1)
    INSERT(A, n)
{% endhighlight %}

**Pseudo-code #2:** `INSERT(A, k)`

{% highlight java linenos %}
key = A[k]
index = k - 1
while index > 0 and A[index] > key
    A[index + 1] = A[index]
    index = index - 1
A[index + 1] = key
{% endhighlight %}

**Solution to the Recurrence:** Let us assume that for $$n = 1$$, $$T(n) = c_1$$, where $$c_1$$ is some constant. And on average for $$n > 1$$, inserting an element in its proper position in a sorted array requires shifting half of the elements, i.e. $$c_2n/2 + c_3$$ time ($$c_2n/2$$ for shifting the elements and $$c_3$$ for inserting the element).

So, we can rewrite the recurrence as:

$$T(n) = \begin {cases}
    c_1                        & \text { if } n = 1, \\
    T(n - 1) + c_2(n - 1)/2 + c_3    & \text { if } n > 1
\end {cases}$$

So for any general $$n > 1$$,

$$\begin {align}
T(n) & = T(n - 1) + c_2(n - 1)/2 + c_3 \\
     & = T(n - 2) + c_2(n - 2)/2 + c_3 + \{c_2(n - 1)/2 + c_3\} \\
     & = T(1) + \cdot \cdot \cdot + \{c_2(n - 2)/2 + c_3\} + \{c_2(n - 1)/2 + c_3\} \\
     & = c_1 + \frac {c_2} 2 \{1 + 2 + \cdot \cdot \cdot + (n - 1)\} + c_3(n - 1) \\
     & = c_1 + \frac {c_2} 2 \cdot \frac {n(n - 1)} 2 + c_3(n - 1) \\
     & = \Theta(n^2)
\end {align}$$