---
title:      Exercise 4.3-7
clrs:       [4, 3]
date:       2012-08-28 20:30
---

>Using the master method in Section 4.5, you can show that the solution to the recurrence $$T(n) = 4T(n/3) + n$$ is $$T(n) = \Theta(n^{\log_3 4})$$. Show that a substitution proof with the assumption $$T(n) \le cn^{\log_3 4}$$ fails. Then show how to subtract off a lower-order term to make a substitution proof work.

Let us assume $$T(n) \le cn^{\log_3 4}$$ for all $$n \ge n_0$$, where $$c$$ and $$n_0$$ are positive constants.

$$\begin {align}
T(n) & \le 4c\left( \frac n 3\right)^{\log_3 4} + n \\
     & \le cn^{\log_3 4} + n
\end {align}$$

We cannot proceed further with this.

Now, let us assume $$T(n) \le cn^{\log_3 4} - n$$ for all $$n \ge n_0$$, where $$c$$ and $$n_0$$ are positive constants.

$$\begin {align}
T(n) & \le 4c\left( \frac n 3\right)^{\log_3 4} - 4n + n \\
     & \le cn^{\log_3 4} - 3n \\
     & \le cn^{\log_3 4} - n
\end {align}$$

Hence, our assumption is correct.