---
title:      Exercise 4.3-8
clrs:       [4, 3]
date:       2012-08-28 20:35
---

>Using the master method in Section 4.5, you can show that the solution to the recurrence $$T(n) = 4T(n/2) + n^2$$ is $$T(n) = \Theta(n^2)$$. Show that a substitution proof with the assumption $$T(n) \le cn^2$$ fails. Then show how to subtract off a lower-order term to make a substitution proof work.

Let us assume $$T(n) \le cn^2$$ for all $$n \ge n_0$$, where $$c$$ and $$n_0$$ are positive constants.

$$\begin {align}
T(n) & \le 4c\left( \frac n 2\right)^2 + n^2 \\
     & = cn^2 + n^2
\end {align}$$

With this we cannot prove our assumption in it's exact form.

Now, let us assume $$T(n) \le cn^2 - n$$ for all $$n \ge n_0$$, where $$c$$ and $$n_0$$ are positive constants.

$$\begin {align}
T(n) & \le 4\left(c\left( \frac n 2\right)^2 - \frac n 2\right) + n^2 \\
     & = 4\left(c\frac {n^2} 4 - \frac n 2\right) + n^2 \\
     & = cn^2 - 2n + n^2 \\
     & = cn^2 - n - n + n^2 \\
     & = cn^2 - n - n(1 - n)
\end {align}$$

Uh oh! From this we cannot say the last step will be less than or equal to $$cn^2 - n$$ when $$n$$ is sufficiently large.

So, what does that mean?
This means we are trying to prove a wrong assumption. And if you use Master Theorem, you will see the asymptotic bound of the given recurrence is $$\Theta(n^2 \lg n)$$, not $$\Theta(n^2)$$ as given in the problem statement.

So, let us assume $$T(n) \le cn^2 \lg n - n$$ for all $$n \ge n_0$$, where $$c$$ and $$n_0$$ are positive constants.---
title:      Exercise 4.3-8
clrs:       [4, 3]
date:       2012-08-28 20:35
---

>Using the master method in Section 4.5, you can show that the solution to the recurrence $$T(n) = 4T(n/2) + n^2$$ is $$T(n) = \Theta(n^2)$$. Show that a substitution proof with the assumption $$T(n) \le cn^2$$ fails. Then show how to subtract off a lower-order term to make a substitution proof work.

Let us assume $$T(n) \le cn^2$$ for all $$n \ge n_0$$, where $$c$$ and $$n_0$$ are positive constants.

$$\begin {align}
T(n) & \le 4c\left( \frac n 2\right)^2 + n^2 \\
     & = cn^2 + n^2
\end {align}$$

With this we cannot prove our assumption in it's exact form.

Now, let us assume $$T(n) \le cn^2 - n$$ for all $$n \ge n_0$$, where $$c$$ and $$n_0$$ are positive constants.

$$\begin {align}
T(n) & \le 4\left(c\left( \frac n 2\right)^2 - \frac n 2\right) + n^2 \\
     & = 4\left(c\frac {n^2} 4 - \frac n 2\right) + n^2 \\
     & = cn^2 - 2n + n^2 \\
     & = cn^2 - n - n + n^2 \\
     & = cn^2 - n - n(1 - n)
\end {align}$$

Uh oh! From this we cannot say the last step will be less than or equal to $$cn^2 - n$$ when $$n$$ is sufficiently large.

So, what does that mean?
This means we are trying to prove a wrong assumption. And if you use Master Theorem, you will see the asymptotic bound of the given recurrence is $$\Theta(n^2 \lg n)$$, not $$\Theta(n^2)$$ as given in the problem statement.

So, let us assume $$T(n) \le cn^2 \lg n - n$$ for all $$n \ge n_0$$, where $$c$$ and $$n_0$$ are positive constants.