---
title:      Problem 3-1
clrs:       [3, 0]
date:       2012-08-25 23:00
---

>***Asymptotic behavior of polynomials***
>
>Let
>
>$$p(n) = \sum_{i = 0}^d a_in^i$$
>
>where $$a_d > 0$$, be a degree-$$d$$ polynomial in $$n$$, and let $$k$$ be a constant. Use the
definitions of the asymptotic notations to prove the following properties.
>
>1. If $$k \ge d$$, then $$p(n) = O(n^k)$$.
<br/>
2. If $$k \le d$$, then $$p(n) = \Omega(n^k)$$.
<br/>
3. If $$k = d$$, then $$p(n) = \Theta(n^k)$$.
<br/>
4. If $$k > d$$, then $$p(n) = o(n^k)$$.
<br/>
5. If $$k < d$$, then $$p(n) = \omega(n^k)$$.

<b>1. Asymptotic Upper Bound</b>

To show that $$p(n) = O(n^k)$$ when $$k \ge d$$, we have to show there exists constants $$c, n_0 > 0$$ such that $$0 \le p(n) \le c \cdot n^k$$ for all $$n \ge n_0$$.

$$\begin {align}
p(n) & = \sum_{i = 0}^d a_in^i \\
     & = a_0 + a_1n^1 + a_2n^2 + \cdots + a_dn^d + \cdots + a_dn^d \\
     & \le \sum_{i = 0}^d a_i
\end {align}$$

The last line follows from the fact that as $$k \ge d$$, for all possible values of $$i$$, $$(i - k) \le 0$$, i.e. all $$n^{i - k}$$ will be less than or equal to 1 for all $$n \ge 1$$.

So we can say that $$0 \le p(n) \le c \cdot n^k$$, where $$c = \sum_{i = 0}^d a_i$$ and $$n_0 = 1$$.

Hence, $$p(n) = O(n^k)$$.

<b>2. Asymptotic Lower Bound</b>

To show that $$p(n) = \Omega(n^k)$$ when $$k \le d$$, we have to show there exists constants $$c, n_0 > 0$$ such that $$0 \le c \cdot n^k \le p(n)$$ for all $$n \ge n_0$$.

$$\begin {align}
p(n) & = \sum_{i = 0}^d a_in^i \\
     & = a_0 + a_1n + a_2n^2 + \cdots + a_kn^k + \cdots + a_dn^d \\
     & \ge a_kn^k
\end {align}$$

So we can say that $$0 \le c \cdot n^k \le p(n)$$, where $$c = a_k$$ and $$n_0 = 1$$.

Hence, $$p(n) = \Omega(n^k)$$.

<b>3. Asymptotic Bound</b>

We have already proved that for $$k = d$$, $$p(n) = O(n)$$ and $$p(n) = \Omega(n)$$. Hence, $$p(n) = \Theta(n)$$.

<b>4. Asymptotic Tight Upper Bound</b>

We can easily prove this by removing the equality from the proof of 1.

Other than that we can use the limit definition of $$o$$-notation:

$$\begin {align}
\lim_{n \to \infty} \frac {p(n)} {n^k} & = \lim_{n \to \infty} \frac {\sum_{i = 0}^d a_in^i} {n^k} \\
& = \lim_{n \to \infty} \frac {a_dn^d} {n^k} \\
& = 0 \qquad(\text { as } k > d)
\end {align}$$

Hence, $$p(n) = o(n)$$.

<b>5. Asymptotic Tight Lower Bound</b>

We can easily prove this by removing the equality from the proof of 2.

Other than that we can use the limit definition of $$\omega$$-notation:

$$\begin {align}
\lim_{n \to \infty} \frac {p(n)} {n^k} & = \lim_{n \to \infty} \frac {\sum_{i = 0}^d a_in^i} {n^k} \\
& = \lim_{n \to \infty} \frac {a_dn^d} {n^k} \\
& = \infty \qquad(\text { as } k < d)
\end {align}$$

Hence, $$p(n) = \omega(n)$$.