---
title:      Exercise 3.1-5
clrs:       [3, 1]
date:       2012-08-25 18:25
---

>Prove Theorem 3.1.
>
>For any two functions $$f(n)$$ and $$g(n)$$, we have $$f(n) = \Theta(g(n))$$ if and only if $$f(n) = O(g(n))$$ and $$f(n) = \Omega(g(n))$$.

To prove this theorem, we need to show the logic holds both ways.

If $$f(n) = \Theta(g(n))$$, then $$0 \le c_1 g(n) \le f(n) \le c_2 g(n)$$ for $$n \ge n_0$$.
As $$0 \le f(n) \le c_2 g(n)$$ for $$n \ge n_0$$, $$f(n) = O(g(n))$$.
And as $$0 \le c_1 g(n) \le f(n)$$ for $$n \ge n_0$$, $$f(n) = \Omega(g(n))$$.

<br/>
Now we need to prove the other way around.

If $$f(n) = \Omega(g(n))$$, then $$0 \le c_1 g(n) \le f(n)$$ for $$n \ge n_1$$.
And if $$f(n) = O(g(n))$$, then $$0 \le f(n) \le c_2 g(n)$$ for $$n \ge n_2$$.

Combining the above two inequalities, we can say $$0 \le c_1 g(n) \le f(n)$$ for $$n \ge max(n_1, n_2)$$, i.e. $$f(n) = \Theta(g(n))$$.