---
title:      Exercise 3.1-2
clrs:       [3, 1]
date:       2012-08-25 18:05
---

>Show that for any real constants $$a$$ and $$b$$, where $$b > 0$$, $$(n + a)^b =\Theta(n^b)$$.

To prove this, we have to show that there exists constants $$c_1, c_2, n_0 > 0$$ such that $$0 \le c_1 n^b \le (n + a)^b \le c_2 n^b$$ for all $$n \ge n_0$$.

<br/>
Note that, $$n + a \le 2n$$, when $$|a| \le n$$
Also note, $$n + a \ge \frac 1 2 n$$, when $$|a| \le \frac n 2$$

Therefore, when $$n \ge 2 \vert a \vert$$,

$$0 \le \frac n 2 \le n + a \le 2n$$

As $$b > 0$$, we can raise all the terms of the previous inequality to the power of $$b$$ without breaking the inequality:

$$\begin {align}
0 \le (\frac n 2)^b & \le (n + a)^b \le (2n)^b \\
\Rightarrow 0 \le \frac 1 {2^b}n^b & \le (n + a)^b \le 2^bn^b
\end {align}$$

So, $$(n + a)^b = \Theta(n^b)$$ because there exists $$c_1 = 1/{2^b}$$, $$c_2 = 2^b$$, and $$n_0 = 2 \vert a \vert$$.