---
title:      Exercise 3.2-6
clrs:       [3, 2]
date:       2012-08-25 19:25
---

>Prove by induction that the $$i$$-th Fibonacci number satisfies the equality
>
>$$F_i = \frac {\phi^i − \hat{\phi^i}} {\sqrt 5}$$
>
>where $$\phi$$ is the golden ratio and $$\hat\phi$$ is its conjugate.

From chapter text, the values of $$\phi$$ and $$\hat\phi$$ are as follows:

$$\phi = \frac {1 + \sqrt 5} 2 \qquad \hat\phi = \frac {1 - \sqrt 5} 2$$

And, Fibonacci series is defined by:

$$\begin {align}
F_i = \begin {cases}
    0 & \text { for } i = 0 \\
    1 & \text { for } i = 1 \\
    F_{i-1} + F_{i-2} & \text { for } i \ge 2
\end {cases} \end {align}$$

<u><b>Basis:</b></u>

$$\begin {align}
F_0 & = \frac {\phi^0 − \hat{\phi^0}} {\sqrt 5} = \frac {1 - 1} {\sqrt 5} = 0 \\[2ex]
F_1 & = \frac {\phi^1 − \hat{\phi^1}} {\sqrt 5} = \frac {\sqrt 5} {\sqrt 5} = 1
\end {align}$$

So, the equality holds for the basis steps.

<u><b>Inductive Step:</b></u>